Add more privileged instructions. Make the Asmgen pass generate more of these privileged instructions. Fix the correctness proof of this pass

riscV/Asmgen.v
@@ -723,15 +723,16 @@ Definition indexed_memory_access
         Pluiw X31 hi :: Paddw X31 base X31 :: mk_instr X31 (Ofsimm (Ptrofs.of_int lo)) :: k
     end.
 
-Definition loadind (base: ireg) (ofs: ptrofs) (ty: typ) (dst: mreg) (k: code) :=
+(* The [priv] parameter is used to determine is this is a parameter load or not *)
+Definition loadind (base: ireg) (ofs: ptrofs) (ty: typ) (dst: mreg) (k: code) (priv: bool) :=
   match ty, preg_of dst with
-  | Tint,    IR rd => OK (indexed_memory_access (fun i o => Plw rd i o false) base ofs k)
-  | Tlong,   IR rd => OK (indexed_memory_access (fun i o => Pld rd i o false) base ofs k)
-  | Tsingle, FR rd => OK (indexed_memory_access (Pfls rd) base ofs k)
-  | Tfloat,  FR rd => OK (indexed_memory_access (Pfld rd) base ofs k)
-  | Tany32,  IR rd => OK (indexed_memory_access (fun i o => Plw_a rd i o false) base ofs k)
-  | Tany64,  IR rd => OK (indexed_memory_access (fun i o => Pld_a rd i o false) base ofs k)
-  | Tany64,  FR rd => OK (indexed_memory_access (Pfld_a rd) base ofs k)
+  | Tint,    IR rd => OK (indexed_memory_access (fun i o => Plw rd i o priv) base ofs k)
+  | Tlong,   IR rd => OK (indexed_memory_access (fun i o => Pld rd i o priv) base ofs k)
+  | Tsingle, FR rd => OK (indexed_memory_access (fun i o => Pfls rd i o priv) base ofs k)
+  | Tfloat,  FR rd => OK (indexed_memory_access (fun i o => Pfld rd i o priv) base ofs k)
+  | Tany32,  IR rd => OK (indexed_memory_access (fun i o => Plw_a rd i o priv) base ofs k)
+  | Tany64,  IR rd => OK (indexed_memory_access (fun i o => Pld_a rd i o priv) base ofs k)
+  | Tany64,  FR rd => OK (indexed_memory_access (fun i o => Pfld_a rd i o priv) base ofs k)
   | _, _           => Error (msg "Asmgen.loadind")
   end.
 
@@ -747,8 +748,8 @@ Definition storeind (src: mreg) (base: ireg) (ofs: ptrofs) (ty: typ) (k: code) :
   | _, _           => Error (msg "Asmgen.storeind")
   end.
 
-Definition loadind_ptr (base: ireg) (ofs: ptrofs) (dst: ireg) (k: code) :=
-  indexed_memory_access (if Archi.ptr64 then fun i o => Pld dst i o false else fun i o => Plw dst i o false) base ofs k.
+Definition loadind_ptr (base: ireg) (ofs: ptrofs) (dst: ireg) (k: code) (priv: bool):=
+  indexed_memory_access (if Archi.ptr64 then fun i o => Pld dst i o priv else fun i o => Plw dst i o priv) base ofs k.
 
 Definition storeind_ptr (src: ireg) (base: ireg) (ofs: ptrofs) (k: code) :=
   indexed_memory_access (if Archi.ptr64 then Psd src else Psw src) base ofs k.
@@ -793,10 +794,10 @@ Definition transl_load (chunk: memory_chunk) (addr: addressing)
       transl_memory_access (fun i o => Pld r i o false)  addr args k
   | Mfloat32 =>
       do r <- freg_of dst;
-      transl_memory_access (Pfls r) addr args k
+      transl_memory_access (fun i o => Pfls r i o false) addr args k
   | Mfloat64 =>
       do r <- freg_of dst;
-      transl_memory_access (Pfld r) addr args k
+      transl_memory_access (fun i o => Pfld r i o false) addr args k
   | _ =>
       Error (msg "Asmgen.transl_load")
   end.
@@ -830,7 +831,7 @@ Definition transl_store (chunk: memory_chunk) (addr: addressing)
 
 Definition make_epilogue (f: Mach.function) (k: code) :=
   loadind_ptr SP f.(fn_retaddr_ofs) RA
-    (Pfreeframe f.(fn_stacksize) f.(fn_link_ofs) :: k).
+    (Pfreeframe f.(fn_stacksize) f.(fn_link_ofs) :: k) false.
 
 (** Translation of a Mach instruction. *)
 
@@ -838,14 +839,14 @@ Definition transl_instr (f: Mach.function) (i: Mach.instruction)
                         (ep: bool) (k: code) :=
   match i with
   | Mgetstack ofs ty dst =>
-      loadind SP ofs ty dst k
+      loadind SP ofs ty dst k false
   | Msetstack src ofs ty =>
       storeind src SP ofs ty k
   | Mgetparam ofs ty dst =>
       (* load via the frame pointer if it is valid *)
-      do c <- loadind X30 ofs ty dst k;
+      do c <- loadind X30 ofs ty dst k true;
       OK (if ep then c
-                else loadind_ptr SP f.(fn_link_ofs) X30 c)
+                else loadind_ptr SP f.(fn_link_ofs) X30 c true)
   | Mop op args res =>
       transl_op op args res k
   | Mload chunk addr args dst =>
